git-svn-id: https://projects.brucker.ch/hol-testgen/svn/HOL-TestGen/trunk/hol-testgen@9355 3260e6d1-4efc-4170-b0a7-36055960796d

OCL_core.thy
@@ -121,6 +121,7 @@ begin
             qed
 end
 
+
 instantiation   option  :: (bot)null
 begin 
    definition null_option_def: "(null::'a\<Colon>bot option) \<equiv>  \<lfloor> bot \<rfloor>"
@@ -879,25 +880,30 @@ by(auto simp: not_def OclValid_def true_def invalid_def defined_def false_def
                  bot_fun_def bot_option_def null_fun_def null_option_def
         split: bool.split_asm HOL.split_if_asm option.split option.split_asm)
 
-nitpick_params
- [timeout = 30, tac_timeout = 0.5, show_datatypes,assms=true]
-lemma ocl_and_defargs: 
-"\<tau> \<Turnstile> (P and Q) \<Longrightarrow> (\<tau> \<Turnstile> \<delta> P) \<and> (\<tau> \<Turnstile> \<delta> Q)"
-by(auto dest: foundation5 foundation6)
-
-(*
-nitpick_params
-nitpick_params
- [timeout = 30, tac_timeout = 0.5, show_datatypes]
-lemma ocl_and_defargs: 
-"\<tau> \<Turnstile> ((P and Q)  \<triangleq>  (P or Q))"
-nitpick[show_all]
-
-oops
-lemma "P & Q = Q"
-nitpick
-*)
-
 text{* So far, we have only one strict Boolean predicate (-family): The strict equality. *}
+
+section{*Miscellaneous: OCL's if then else endif *}
+
+
+definition if_ocl :: "[('\<AA>)Boolean , ('\<AA>,'\<alpha>::null) val, ('\<AA>,'\<alpha>) val] \<Rightarrow> ('\<AA>,'\<alpha>) val"
+                     ("if (_) then (_) else (_) endif" [10,10,10]50)
+where "(if C then B\<^isub>1 else B\<^isub>2 endif) = (\<lambda> \<tau>. if (\<delta> C) \<tau> = true \<tau> 
+                                           then (if (C \<tau>) = true \<tau> 
+                                                then B\<^isub>1 \<tau> 
+                                                else B\<^isub>2 \<tau>)
+                                           else invalid \<tau>)"
+
+lemma if_ocl_invalid : "(if invalid then B\<^isub>1 else B\<^isub>2 endif) = invalid"
+by(rule ext, auto simp: if_ocl_def)
+
+lemma if_ocl_null : "(if null then B\<^isub>1 else B\<^isub>2 endif) = invalid"
+by(rule ext, auto simp: if_ocl_def)
+
+lemma if_ocl_true : "(if true then B\<^isub>1 else B\<^isub>2 endif) = B\<^isub>1"
+by(rule ext, auto simp: if_ocl_def)
+
+lemma if_ocl_false : "(if false then B\<^isub>1 else B\<^isub>2 endif) = B\<^isub>2"
+by(rule ext, auto simp: if_ocl_def)
+
 
 end
